[Interpreter] Done.

Lustrean/Interpreter.lean
@@ -7,7 +7,7 @@ inductive inst (n : Nat) : Type :=
 | guard : bexpr n → inst n
 
 namespace Array
-  def All {α : Type} (P : α → Prop) (as : Array α): Prop :=
+  def All {α : Type} (P : α → Prop) (as : Array α) : Prop :=
     ∀ (i : Fin as.size), P (as.get i)
 
   instance {α : Type} (P : α → Prop) [DecidablePred P] (as : Array α) :
@@ -92,40 +92,6 @@ namespace Array
     (f : ∀ (a : α), P a → β) : Array β
   := foldp as P HAll (fun acc a p => acc.push (f a p)) #[]
 
-  theorem mapp_size : ∀ (α β : Type) (as : Array α) (P : α → Prop) (HAll : All P as)
-    (f : ∀ (a : α), P a → β), (mapp as P HAll f).size = as.size
-  := by
-    intros α β as P HAll f
-    unfold mapp foldp foldip foldip.proof_1
-
-    have : ∀ (α β : Type) (P : α → Prop) (n : Nat) (as : Array α) (HAll : All P as)
-      (f : ∀ (a : α), P a → β), as.size = n → (mapp as P HAll f).size = n :=
-    by
-      intros α β P n as HAll f Hn
-      unfold mapp foldp foldip foldip.aux
-      simp
-      induction n
-      case zero =>
-
-      cases Hn
-      symm at Hn
-      cases Hn
-
-
-      rw [Hn]
-
-      simp_all only [eq_mpr_eq_cast, Nat.add_one_sub_one, eq_mp_eq_cast, cast_cast, Array.get_eq_getElem]
-      induction n
-      case zero =>
-        simp
-        sorry
-      case succ n IH =>
-        simp_all only [Nat.add_right_eq_self, Nat.add_one_ne_zero, false_implies]
-        sorry
-    intros α β as P HAll f
-    apply this
-    rfl
-
   def foldi {α : Type} (as : Array α) {β : Type} (f : Fin as.size → β → α → β) (init : β) : β :=
     foldip as (fun _ => True) (fun _ => True.intro) (fun i b a _ => f i b a) init
 end Array
@@ -168,205 +134,350 @@ namespace List
       constructor
 end List
 
-structure pre_node (n : Nat) : Type where
+structure PreNode (nb_var : Nat) : Type where
   id : Nat
-  out_nodes : List (Nat × inst n)
+  out_nodes : List (Nat × inst nb_var)
 
-structure node (n : Nat) (nb_nodes : Nat) : Type where
-  out_nodes : List (Fin nb_nodes × inst n)
+structure Node (nb_var nb_arcs : Nat) : Type where
+  in_nodes : List (Fin nb_arcs)
 
-def get_nodes {nb_var : Nat} (l : List (pre_node nb_var)) : Option ({ arr : Array (node nb_var l.length) // arr.size = l.length }) :=
-  let lsorted := l.mergeSort (fun n₁ n₂ => if n₁.id ≤ n₂.id then true else false)
-  let as := Array.mk lsorted
-  if h : ∀ (i : Fin as.size), (as.get i).id = i ∧ (
-    ∀ p, p ∈ (as.get i).out_nodes → p.fst < l.length
-  )
-  then
-    let Hlength : l.length = as.size := by
-      rw [←Array.data_length]
-      simp
-      rw [List.mergeSort_length]
-    let arr := Array.mapp as (fun a => a.id < l.length ∧ (
-      ∀ p, p ∈ a.out_nodes → p.fst < l.length
-    )) (by
-      intros i
-      specialize h i
-      constructor
-      · rw [h.left, Hlength]
-        apply i.isLt
-      · apply h.right
-    ) (fun pn Hi =>
-      let Hall : ∀ x, x ∈ pn.out_nodes → x.fst < l.length := Hi.right
-      let l := List.foldip pn.out_nodes (fun x => x.fst < l.length) Hall (fun l x Hx =>
-        (Fin.mk x.fst Hx, x.snd) :: l
-      ) []
-      node.mk l
-    )
-    let Harr : arr.size = l.length := by
-      simp [Hlength]
-      simp [arr]
-      apply Array.mapp_size
-    .some ⟨ arr, Harr ⟩
-  else none
-
-structure cfg : Type where
-  nb_var : Nat
-  nb_nodes : Nat
-  nodes : Array (node nb_var nb_nodes)
-  Heq : nodes.size = nb_nodes
-
-structure arc (nb_var : Nat) (nb_nodes : Nat) : Type where
+structure Arc (nb_var nb_nodes : Nat) : Type where
   src : Fin nb_nodes
   dst : Fin nb_nodes
   inst : inst nb_var
 
-namespace cfg
-  def new {nb_var : Nat} (l : List (pre_node nb_var)) : Option cfg :=
-    match get_nodes l with
-    | .none => .none
-    | .some ⟨ nodes, Hnodes ⟩ => cfg.mk nb_var l.length nodes Hnodes
+structure Cfg (nb_var : Nat) : Type where
+  nb_nodes : Nat
+  nb_arcs : Nat
+  nodes : Array (Node nb_var nb_arcs)
+  Hnodes : nb_nodes = nodes.size
+  arcs : Array (Arc nb_var nb_nodes)
+  Harcs : nb_arcs = arcs.size
 
-  def arcs (cfg : cfg) :
-    Array (arc cfg.nb_var cfg.nb_nodes)
-  :=
-    let l : List (arc cfg.nb_var cfg.nb_nodes) :=
-    Array.foldi cfg.nodes  (fun i acc n =>
-      let new : List (arc cfg.nb_var cfg.nb_nodes)
-      := List.map (fun (x : Fin cfg.nb_nodes × inst cfg.nb_var) =>
-        arc.mk /-(TODO: match cfg.Heq with | Eq.refl _ => i)-/
-        /-(Eq.rec i cfg.Heq)-/
-        (by
-          rw [cfg.Heq] at i
-          exact i
-        )
-         x.fst x.snd
-      ) n.out_nodes
-      new ++ acc
-    ) []
-    Array.mk l
+namespace Cfg
+  variable {nb_var : Nat}
+
+  namespace new
+    variable (nb_nodes nb_arcs : Nat)
+
+    def find_nb_arcs (l : List (PreNode nb_var)) : Nat :=
+      List.foldl (fun n pn => n + pn.out_nodes.length) 0 l
+
+    theorem find_nb_arcs_incr : ∀ (l : List (PreNode nb_var)) (n m : Nat),
+      n ≤ m →
+      List.foldl (fun n pn => n + pn.out_nodes.length) n l ≤
+        List.foldl (fun n pn => n + pn.out_nodes.length) m l
+    := by
+      intros l
+      induction l <;> intros n m H
+      case nil => assumption
+      case cons _ _ IH =>
+        apply IH
+        simp
+        assumption
+
+    theorem find_nb_arcs_add : ∀ (l : List (PreNode nb_var)) (n m : Nat),
+      List.foldl (fun n pn => n + pn.out_nodes.length) n l + m
+        = List.foldl (fun n pn => n + pn.out_nodes.length) (n + m) l
+    := by
+      intros l
+      induction l <;> intros n m <;> simp
+      case cons pn' l IH =>
+        rw [IH]
+        have : n + pn'.out_nodes.length + m = n + m + pn'.out_nodes.length := by
+          conv =>
+            lhs
+            rw [Nat.add_assoc]
+            arg 2
+            rw [Nat.add_comm]
+          rw [←Nat.add_assoc]
+        rw [this]
+
+    theorem find_nb_arcs_cons : ∀ (l : List (PreNode nb_var)) (pn : PreNode nb_var),
+      find_nb_arcs l + pn.out_nodes.length = find_nb_arcs (pn :: l) :=
+    by
+      intros l pn
+      simp [find_nb_arcs, find_nb_arcs_add]
+
+    structure NewAux (nb_var nb_nodes nb_arcs : Nat) (l : List (PreNode nb_var)) : Type where
+      nodes : Array (Node nb_var nb_arcs)
+      Hnodes : nb_nodes = nodes.size
+      arcs : Array (Arc nb_var nb_nodes)
+      Harcs : find_nb_arcs l = arcs.size
+
+    def init : NewAux nb_var nb_nodes nb_arcs [] :=
+      .mk (Array.mkArray nb_nodes (.mk [])) (by simp) #[] rfl
+
+    structure StepAux (nb_var nb_nodes nb_arcs : Nat)
+      (l : List (PreNode nb_var))
+      (out : List (Nat × inst nb_var)) : Type
+    where
+      nodes : Array (Node nb_var nb_arcs)
+      Hnodes : nb_nodes = nodes.size
+      arcs : Array (Arc nb_var nb_nodes)
+      Harcs : find_nb_arcs l + out.length = arcs.size
+
+    def step.init (l : List (PreNode nb_var))
+      (cfg : NewAux nb_var nb_nodes nb_arcs l) :
+      StepAux nb_var nb_nodes nb_arcs l []
+    := .mk cfg.nodes cfg.Hnodes cfg.arcs cfg.Harcs
+
+    def step.aux (l : List (PreNode nb_var)) (i : Fin nb_nodes)
+      (out_node : Nat)
+      (out_inst : inst nb_var)
+      (Hout : out_node < nb_nodes)
+      (out_nodes : List (Nat × inst nb_var))
+      (Harcs : find_nb_arcs l + out_nodes.length < nb_arcs)
+      (cfg : StepAux nb_var nb_nodes nb_arcs l out_nodes) :
+      StepAux nb_var nb_nodes nb_arcs l ((out_node, out_inst) :: out_nodes)
+    :=
+      let dst := .mk out_node Hout
+      let arc := .mk i dst out_inst
+      let H : cfg.arcs.size < nb_arcs := by
+        rw [←cfg.Harcs]
+        assumption
+      let arc_idx := .mk cfg.arcs.size H
+      let arcs := cfg.arcs.push arc
+      let Harcs : find_nb_arcs l + ((out_node, out_inst) :: out_nodes).length = arcs.size := by
+        simp [arcs, ←Nat.add_assoc]
+        apply cfg.Harcs
+      let old_in_arcs := (cfg.nodes.get (cfg.Hnodes ▸ dst)).in_nodes
+      let new_node := .mk (arc_idx :: old_in_arcs)
+      let nodes := cfg.nodes.set (cfg.Hnodes ▸ dst) new_node
+      let Hnodes : nb_nodes = nodes.size := by
+        simp [nodes, cfg.Hnodes]
+      .mk nodes Hnodes arcs Harcs
+
+    def step.run (l : List (PreNode nb_var)) (i : Fin nb_nodes)
+      (out_nodes : List (Nat × inst nb_var))
+      (Hn : ∀ p, p ∈ out_nodes → p.fst < nb_nodes)
+      (Harcs : find_nb_arcs l + out_nodes.length ≤ nb_arcs)
+      (cfg : NewAux nb_var nb_nodes nb_arcs l) :
+      StepAux nb_var nb_nodes nb_arcs l out_nodes
+    := match out_nodes with
+    | [] => step.init nb_nodes nb_arcs l cfg
+    | (out_node, out_inst) :: out_nodes =>
+      let Hl : find_nb_arcs l + out_nodes.length ≤ nb_arcs := by
+        simp at Harcs
+        rw [←Nat.add_assoc] at Harcs
+        apply Nat.le_trans
+        · apply Nat.le_succ
+        · assumption
+      let cfg := step.run l i out_nodes (by
+        intros p Hp
+        apply Hn
+        simp [Hp]
+      ) Hl cfg
+      step.aux nb_nodes nb_arcs l i out_node out_inst (by
+        let H := Hn (out_node, out_inst)
+        simp at H
+        assumption
+      ) out_nodes Harcs cfg
+
+    def step (l : List (PreNode nb_var))
+      (i : Fin nb_nodes) (cfg : NewAux nb_var nb_nodes nb_arcs l)
+    (pn : PreNode nb_var) (Hn : pn.id = i ∧ (
+      ∀ p, p ∈ pn.out_nodes → p.fst < nb_nodes
+    ))
+    (Harcs : find_nb_arcs l + pn.out_nodes.length ≤ nb_arcs)
+    : NewAux nb_var nb_nodes nb_arcs (pn :: l)
+    :=
+      let cfg := step.run nb_nodes nb_arcs l i pn.out_nodes Hn.right Harcs cfg
+      let Heq : find_nb_arcs l + pn.out_nodes.length = find_nb_arcs (pn :: l) := by
+        apply find_nb_arcs_cons
+      .mk cfg.nodes cfg.Hnodes cfg.arcs (Heq ▸ cfg.Harcs)
+
+    def aux (l : List (PreNode nb_var))
+      (Hlength : List.length l ≤ nb_nodes)
+      (Harcs : find_nb_arcs l ≤ nb_arcs)
+      (Hsorted : ∀ (i : Fin l.length), (l.get i).id = (i + nb_nodes - List.length l) ∧ (
+        ∀ p, p ∈ (l.get i).out_nodes → p.fst < nb_nodes
+      )) : NewAux nb_var nb_nodes nb_arcs l
+    := match l with
+    | [] => init nb_nodes nb_arcs
+    | pn :: l =>
+      let Ha : find_nb_arcs l ≤ nb_arcs := by
+        simp [find_nb_arcs] at Harcs
+        simp [find_nb_arcs]
+        apply Nat.le_trans
+        · apply find_nb_arcs_incr
+          apply Nat.zero_le pn.out_nodes.length
+        · assumption
+      let Hl : l.length ≤ nb_nodes := by
+        apply Nat.le_trans
+        · apply Nat.le_succ
+        · assumption
+      let cfg := aux l Hl Ha (by
+        intros i
+        let H := Hsorted i.succ
+        simp at Hlength
+        have Hl' : l.length + 1 ≤ nb_nodes + 1 := by
+          rw [Nat.add_le_add_iff_right]
+          assumption
+        have : i + nb_nodes - l.length = i.succ + nb_nodes - (pn :: l).length := by
+          simp
+          conv =>
+            rhs
+            rw [Nat.add_assoc]
+            lhs
+            rhs
+            rw [Nat.add_comm]
+          conv =>
+            rhs
+            rw [Nat.add_sub_assoc Hl']
+            simp
+            rw [←Nat.add_sub_assoc Hl]
+        simp at H
+        simp
+        rw [this]
+        assumption
+      )
+      let i : Fin nb_nodes := .mk (nb_nodes - List.length (pn :: l)) <| by
+        simp [Hsorted]
+        apply Nat.sub_lt
+        · apply Nat.le_trans
+          · apply Nat.zero_lt_succ l.length
+          · assumption
+        · simp
+      let Heq : find_nb_arcs l + pn.out_nodes.length = find_nb_arcs (pn :: l) := by
+        apply find_nb_arcs_cons
+      step nb_nodes nb_arcs l i cfg pn (by
+        simp at Hsorted
+        let H := Hsorted 0
+        simp at H
+        simp
+        assumption
+      ) (Heq ▸ Harcs)
+  end new
+
+  def new (l : List (PreNode nb_var)) : Option (Cfg nb_var) :=
+    let lsorted := l.mergeSort (fun n₁ n₂ => if n₁.id ≤ n₂.id then true else false)
+    if Hsorted : ∀ (i : Fin lsorted.length), (lsorted.get i).id = i ∧ (
+        ∀ p, p ∈ (lsorted.get i).out_nodes → p.fst < lsorted.length
+      )
+    then
+      let nb_arcs := new.find_nb_arcs lsorted
+      let Hl : l.length = lsorted.length := by
+        simp [lsorted, List.mergeSort_length]
+      let aux := new.aux l.length nb_arcs lsorted (by simp [Hl])
+        (by simp [nb_arcs]) <| by
+        rw [Hl]
+        intros i
+        rw [Nat.add_sub_cancel]
+        apply Hsorted
+      .some (.mk l.length nb_arcs aux.nodes aux.Hnodes aux.arcs <| by
+        simp [nb_arcs]
+        apply aux.Harcs
+      )
+    else .none
 
   -- TODO: do better
   -- true : should widen, false : shouldn't
-  def get_widening_points (cfg : cfg) : { arr : Array Bool // arr.size = cfg.nb_nodes }
+  def get_widening_points {nb_var : Nat} (cfg : Cfg nb_var) : { arr : Array Bool // arr.size = cfg.nb_nodes }
   :=
     let arr := Array.mkArray cfg.nb_nodes true
     let Harr : arr.size = cfg.nb_nodes := by
       simp [arr]
     ⟨ arr, Harr ⟩
-end cfg
+end Cfg
 
-structure state (α : Type) [Domain α] (cfg : cfg) where
-  node_env : Array α
+structure State (α : Type) [ι : Domain α] (cfg : Cfg ι.nb_var) where
+  node_env : Array α -- holds an environment at each node
   Hnode_env : node_env.size = cfg.nb_nodes
+  arc_env : Array α -- holds [[arc.inst]](env) for each arc where env is the environment at arc.src
+  Harc_env : arc_env.size = cfg.nb_arcs
+  widening_points : Array Bool
+  Hwidening_points : widening_points.size = cfg.nb_nodes
+  nb_step : Nat
 
-namespace state
-  variable {α : Type} [ι : Domain α] {cfg : cfg} (s : state α cfg)
+namespace State
+  variable {α : Type} [ι : Domain α] {cfg : Cfg ι.nb_var}
 
-  def get (i : Fin cfg.nb_nodes) : α :=
-    s.node_env.get (by -- TODO
-      rw [s.Hnode_env]
-      apply i
-    )
+  def get_node_env (s : State α cfg) (i : Fin cfg.nb_nodes) : α :=
+    s.node_env.get (s.Hnode_env ▸ i)
 
-  def set (i : Fin cfg.nb_nodes) (a : α) : state α cfg :=
-    let node_env := s.node_env.set (by -- TODO
-        rw [s.Hnode_env]
-        apply i
-      ) a
+  def set_node_env (i : Fin cfg.nb_nodes) (a : α) : StateM (State α cfg) Unit := do
+    let s ← get
+    let node_env := s.node_env.set (s.Hnode_env ▸ i) a
     let Hnode_env : node_env.size = cfg.nb_nodes := by
       rw [←s.Hnode_env]
       simp [node_env]
-    state.mk node_env Hnode_env
+    set ({ s with node_env := node_env, Hnode_env := Hnode_env})
 
-  def iter (s : state α cfg) : state α cfg :=
-    let iter_arc (arc : arc cfg.nb_var cfg.nb_nodes) :=
-      let src_env := s.get arc.src
-      let dst_env := match s.get arc.inst with
-      | .skip => src_env
-      | .assign var expr => src_env.assign var expr
-      | .guard b  => src_env.guard b
-    sorry
+  def get_arc_env (s : State α cfg) (i : Fin cfg.nb_arcs) : α :=
+    s.arc_env.get (s.Harc_env ▸ i)
 
+  def set_arc_env (i : Fin cfg.nb_arcs) (a : α) : StateM (State α cfg) Unit := do
+    let mut s ← get
+    let arc_env := s.arc_env.set (s.Harc_env ▸ i) a
+    let Harc_env : arc_env.size = cfg.nb_arcs := by
+      simp [arc_env, s.Harc_env]
+    set ({ s with arc_env := arc_env, Harc_env := Harc_env})
 
-/-  def unique {α : Type} (P : α → Prop) : α → Prop :=
-    fun (a : α) => P a ∧ ∀ (b : α), P b → a = b
+  def iter_arc (arc_idx : Fin cfg.nb_arcs) : StateM (State α cfg) Bool := do
+    let s ← get
+    let arc := cfg.arcs.get (cfg.Harcs ▸ arc_idx)
+    let src_env := s.get_node_env arc.src
+    let old_env := s.get_arc_env arc_idx
+    let new_env := match arc.inst with
+    | .skip => src_env
+    | .assign var expr => ι.assign src_env var expr
+    | .guard b  => ι.guard src_env b
+    set_arc_env arc_idx new_env
+    let _ := ι.eq_dec
+    let _ := ι.is_subset_dec
+    let modified := decide ¬ ι.is_subset old_env new_env
+    return modified
 
-  def dec_forall_fin {n : Nat} (P : Fin n → Prop) [ι : DecidablePred P] :
-    Decidable (∀ (i : Fin n), P i)
-  := by
-    induction n
-    · apply isTrue
-      intros i
-      cases i
-      rename_i v Hv
-      cases Hv
-    · rename_i n IH
-      cases (ι 0) <;> rename_i H
-      · apply isFalse
-        intros Hc
-        apply H
-        apply Hc
-      · cases (IH (fun (i : Fin n) => P i.succ)) <;> rename_i H'
-        · apply isFalse
-          intros Hc
-          apply H'
-          intros i
-          apply Hc
-        · apply isTrue
-          intros j
-          apply Fin.cases <;> assumption
+  def iter_node (node_idx : Fin cfg.nb_nodes) : StateM (State α cfg) Unit := do
+    let s ← get
+    let node := cfg.nodes.get (cfg.Hnodes.symm ▸ node_idx)
+    let in_env := List.foldl (fun acc_env arc_idx =>
+      let env := s.get_arc_env arc_idx
+      ι.join acc_env env
+    ) ι.bot node.in_nodes
+    let s ← get
+    if s.widening_points.get (s.Hwidening_points ▸ node_idx)
+    then
+      let old_env := s.get_node_env node_idx
+      set_node_env node_idx (ι.widen old_env in_env s.nb_step)
+    else
+      set_node_env node_idx in_env
+    return
 
-  instance {n : Nat} (P : Fin n → Prop) [DecidablePred P] :
-    Decidable (∀ (i : Fin n), P i) := dec_forall_fin P
+  def iter : StateM (State α cfg) Bool := do
+    let mut result := false
+    for h : i in [0:cfg.nb_arcs] do
+      let b ← iter_arc <| .mk i <| by
+        apply Membership.get_elem_helper
+        · assumption
+        · rfl
+      result := result || b
+    for h : i in [0:cfg.nb_nodes] do
+      iter_node <| .mk i <| by
+        apply Membership.get_elem_helper
+        · assumption
+        · rfl
+    let s ← get
+    set ({ s with nb_step := s.nb_step.succ })
+    return result
 
-  def dec_exists_fin {n : Nat} (P : Fin n → Prop) [ι : DecidablePred P] :
-    Decidable (∃ (i : Fin n), P i)
-  := by
-    induction n
-    · apply isFalse
-      intros Hc
-      cases Hc
-      rename_i v _
-      cases v
-      rename_i Hc _
-      cases Hc
-    · rename_i n IH
-      cases (ι 0) <;> rename_i H
-      · cases (IH (fun (i : Fin n) => P i.succ)) <;> rename_i H'
-        · apply isFalse
-          have HF : ∀ (i : Fin n.succ), ¬P i := by
-            intros i
-            apply (@Fin.cases n (fun i => ¬P i))
-            · assumption
-            · intros j Hc
-              apply H'
-              exists j
-          intros Hc
-          cases Hc
-          apply HF
-          assumption
-        · apply isTrue
-          cases H'
-          rename_i i _
-          exists i.succ
-      · apply isTrue
-        exists 0
+  partial def loop : StateM (State α cfg) Unit := do
+    let b ← iter
+    if b then loop
 
-  instance {n : Nat} (P : Fin n → Prop) [DecidablePred P] :
-    Decidable (∃ (i : Fin n), P i) := dec_exists_fin P
+  def init : State α cfg :=
+    let node_env := Array.mkArray cfg.nb_nodes ι.bot
+    let Hnode_env : node_env.size = cfg.nb_nodes := by
+      simp [node_env]
+    let arc_env := Array.mkArray cfg.nb_arcs ι.bot
+    let Harc_env : arc_env.size = cfg.nb_arcs := by
+      simp [arc_env]
+    let widening_points := cfg.get_widening_points
+    .mk node_env Hnode_env
+      arc_env Harc_env
+      widening_points.val widening_points.property 0
 
-  def dec_unique_fin {n : Nat} (P : Fin n → Prop) [ι : DecidablePred P] :
-    DecidablePred (unique P)
-  := by
-    intros i
-    unfold unique
-    apply inferInstance
-
-  instance {n : Nat} (P : Fin n → Prop) [DecidablePred P] :
-    DecidablePred (unique P) := dec_unique_fin P
-
-  def exists_unique_fin {n : Nat} (P : Fin n → Prop) [DecidablePred P] :
-    Decidable (∃ (i : Fin n), unique P i) := inferInstance
-
-  instance {n : Nat} (P : Fin n → Prop) [DecidablePred P] :
-    Decidable (∃ (i : Fin n), unique P i) := exists_unique_fin P-/
+  def run (cfg : Cfg ι.nb_var) : State α cfg :=
+    (StateT.run loop init).2
+end State
